Bignum/BitVec.lean
@@ -1,5 +1,5 @@
 /-
-Copyright (c) 2026 Guilherme Lima. All Rights Reserved.
+Copyright (c) 2026 Guilherme Lima. All rights reserved.
 Released under Apache 2.0 license as described in the file LICENSE.
 Author(s): Guilherme Lima.
 -/
