BignumTest/ArmRev/ShiftType.lean
@@ -6,32 +6,42 @@ open Bignum.ArmRev
 
 /-- info: 0x00000008#32 -/
 #guard_msgs in
-#eval ShiftType.LSL.shift 0x4#32 1
+#eval ShiftType.LSL.shift 1 0x4#32
 
 /-- info: 0x00000000#32 -/
 #guard_msgs in
-#eval ShiftType.LSL.shift 0x80000000#32 1
+#eval ShiftType.LSL.shift 1 0x80000000#32
 
 -- LSR
 
 /-- info: 0x00000002#32 -/
 #guard_msgs in
-#eval ShiftType.LSR.shift 0x4#32 1
+#eval ShiftType.LSR.shift 1 0x4#32
 
 /-- info: 0x00000000#32 -/
 #guard_msgs in
-#eval ShiftType.LSR.shift 0x1#32 1
+#eval ShiftType.LSR.shift 1 0x1#32
 
 -- ASR
 
 /-- info: 0x00000000#32 -/
 #guard_msgs in
-#eval ShiftType.ASR.shift 0x0#32 1
+#eval ShiftType.ASR.shift 1 0x0#32
 
 /-- info: 0x00000000#32 -/
 #guard_msgs in
-#eval ShiftType.ASR.shift 0x1#32 1
+#eval ShiftType.ASR.shift 1 0x1#32
 
 /-- info: 0x2#4 -/
 #guard_msgs in
-#eval ShiftType.ASR.shift 0x5#4 1
+#eval ShiftType.ASR.shift 1 0x5#4
+
+-- ROR
+
+/-- info: 0x80#8 -/
+#guard_msgs in
+#eval ShiftType.ROR.shift 1 0x1#8
+
+/-- info: 0x1#4 -/
+#guard_msgs in
+#eval ShiftType.ROR.shift 1 0x2#4
